checkout point before renaming

impl/riscv/mod_pow_lemmas.i.dfy
@@ -8,13 +8,14 @@ module mod_pow_lemmas {
     import opened BASE_32_Seq
     import opened Mul
     import Power2
-    import Power
+    import opened Power
     import opened DivMod
     
+    import opened mont_mul_add_lemmas
     import opened mont_mul_lemmas
 
     datatype mp_vars = mp_vars(
-        me_frame_ptr: uint32, // writable
+        mp_frame_ptr: uint32, // writable
         mm_frame_ptr: uint32, // writable
         mma_frame_ptr: uint32, // writable
         iter_rr: iter_t, 
@@ -36,9 +37,13 @@ module mod_pow_lemmas {
         out_ptr: nat,
         rsa: rsa_params)
     {
+        && valid_frame_ptr(mem, vars.mp_frame_ptr, 8)
+        && valid_frame_ptr(mem, vars.mm_frame_ptr, 8)
+        && valid_frame_ptr(mem, vars.mma_frame_ptr, 12)
+
         && mvar_iter_inv(mem, vars.iter_rr, rr_ptr, 0, rsa.RR)
         && mvar_iter_inv(mem, vars.iter_n, n_ptr, 0, rsa.M)
-        && mvar_iter_inv(mem, vars.iter_in, in_ptr, 0, rsa.M)
+        && mvar_iter_inv(mem, vars.iter_in, in_ptr, 0, rsa.SIG)
         && mvar_iter_inv(mem, vars.iter_ar, ar_ptr, 0, NA)
         && mvar_iter_inv(mem, vars.iter_aar, aar_ptr, 0, NA)
         && mvar_iter_inv(mem, vars.iter_out, out_ptr, 0, NA)
@@ -48,7 +53,7 @@ module mod_pow_lemmas {
         && vars.iter_ar.base_addr != vars.iter_in.base_addr
         && vars.iter_ar.base_addr != vars.iter_aar.base_addr
         && vars.iter_ar.base_addr != vars.iter_out.base_addr
-        && vars.iter_ar.base_addr != vars.me_frame_ptr
+        && vars.iter_ar.base_addr != vars.mp_frame_ptr
         && vars.iter_ar.base_addr != vars.mm_frame_ptr
         && vars.iter_ar.base_addr != vars.mma_frame_ptr
 
@@ -56,22 +61,22 @@ module mod_pow_lemmas {
         && vars.iter_aar.base_addr != vars.iter_n.base_addr
         && vars.iter_aar.base_addr != vars.iter_in.base_addr
         && vars.iter_aar.base_addr != vars.iter_out.base_addr
-        && vars.iter_aar.base_addr != vars.me_frame_ptr
+        && vars.iter_aar.base_addr != vars.mp_frame_ptr
         && vars.iter_aar.base_addr != vars.mm_frame_ptr
         && vars.iter_aar.base_addr != vars.mma_frame_ptr
 
         && vars.iter_out.base_addr != vars.iter_rr.base_addr
         && vars.iter_out.base_addr != vars.iter_n.base_addr
         && vars.iter_out.base_addr != vars.iter_in.base_addr
-        && vars.iter_out.base_addr != vars.me_frame_ptr
+        && vars.iter_out.base_addr != vars.mp_frame_ptr
         && vars.iter_out.base_addr != vars.mm_frame_ptr
         && vars.iter_out.base_addr != vars.mma_frame_ptr
 
-        && vars.me_frame_ptr != vars.iter_rr.base_addr
-        && vars.me_frame_ptr != vars.iter_n.base_addr
-        && vars.me_frame_ptr != vars.iter_in.base_addr
-        && vars.me_frame_ptr != vars.mm_frame_ptr
-        && vars.me_frame_ptr != vars.mma_frame_ptr
+        && vars.mp_frame_ptr != vars.iter_rr.base_addr
+        && vars.mp_frame_ptr != vars.iter_n.base_addr
+        && vars.mp_frame_ptr != vars.iter_in.base_addr
+        && vars.mp_frame_ptr != vars.mm_frame_ptr
+        && vars.mp_frame_ptr != vars.mma_frame_ptr
 
         && vars.mm_frame_ptr != vars.iter_rr.base_addr
         && vars.mm_frame_ptr != vars.iter_n.base_addr
@@ -81,5 +86,68 @@ module mod_pow_lemmas {
         && vars.mma_frame_ptr != vars.iter_rr.base_addr
         && vars.mma_frame_ptr != vars.iter_n.base_addr
         && vars.mma_frame_ptr != vars.iter_in.base_addr
+
+        && rsa_params_inv(rsa)
+    }
+
+    predicate modexp_var_inv(a: seq<uint32>, rsa: rsa_params, i: nat)
+        requires rsa_params_inv(rsa)
+    {
+        LemmaPowPositiveAuto();
+        && IsModEquivalent(to_nat(a), Pow(rsa.SIG, Pow(4, i)) * rsa.R, rsa.M)
+    }
+
+    lemma modexp_var_inv_pre_lemma(
+        a_view: seq<uint32>,
+        rr: seq<uint32>,
+        sig: seq<uint32>,
+        rsa: rsa_params)
+
+    requires montmul_inv(a_view, sig, NUM_WORDS, rr, rsa);
+    requires to_nat(rr) == rsa.RR;
+    requires to_nat(sig) == rsa.SIG;
+    ensures modexp_var_inv(a_view, rsa, 0);
+
+    lemma modexp_var_inv_peri_lemma(
+        ar: seq<uint32>,
+        aar: seq<uint32>,
+        aaaar: seq<uint32>,
+        i: nat,
+        rsa: rsa_params)
+
+        requires montmul_inv(aar, ar, NUM_WORDS, ar, rsa);
+        requires montmul_inv(aaaar, aar, NUM_WORDS, aar, rsa);
+        requires modexp_var_inv(ar, rsa, i);
+        ensures modexp_var_inv(aaaar, rsa, i + 1);
+
+    lemma modexp_var_inv_post_lemma(
+        a_view: seq<uint32>,
+        next_a_view: seq<uint32>,
+        sig: seq<uint32>,
+        rsa: rsa_params)
+
+        requires montmul_inv(next_a_view, a_view, NUM_WORDS, sig, rsa);
+        requires modexp_var_inv(a_view, rsa, 8);
+        ensures IsModEquivalent(to_nat(next_a_view), Pow(to_nat(sig), 65537), rsa.M);
+
+    lemma modexp_var_correct_lemma(
+        raw_val: nat,
+        adjusted_val: nat,
+        carry: bool,
+        rsa: rsa_params)
+
+    requires rsa_params_inv(rsa);
+    requires raw_val < rsa.SIG + rsa.M;
+    requires IsModEquivalent(raw_val, Pow(rsa.SIG, 65537), rsa.M);
+    requires carry ==> raw_val < rsa.M;
+    requires !carry ==> raw_val - rsa.M == adjusted_val;
+
+    ensures carry ==> raw_val == Pow(rsa.SIG, 65537) % rsa.M;
+    ensures !carry ==> adjusted_val == Pow(rsa.SIG, 65537) % rsa.M;
+
+    function mod(a: nat, m: nat): int
+        requires m != 0;
+    {
+        a % m
     }
 }
